started the hpare_sound proof

hoareProofDefScript.sml
@@ -1,7 +1,7 @@
 open HolKernel Parse boolLib bossLib;
-open stringTheory hoareSyntaxDefTheory;
+open stringTheory hoareSyntaxDefTheory  hoareSemanticsDefTheory;
 
-val _ = new_theory "hoareSemanticsDef";
+val _ = new_theory "hoareProofDef";
 
 val _ = type_abbrev("var"  , ``:string``);
 val _ = type_abbrev("env"  , ``:string -> num``);
@@ -16,8 +16,32 @@ End
 Inductive Hoare:
   (Hoare P CSkip P) ∧
   (Hoare (assert_subst Q v ae) (CAsgn v ae) Q) ∧
-  (Hoare P c1 Q ∧ Hoare Q c2 R ⇒ Hoare P (Cseq c1 c2) R)
+  (Hoare P c1 Q ∧ Hoare Q c2 R ⇒ Hoare P (Cseq c1 c2) R) ∧
+  (Hoare (λenv. P env ∧ eval_bexpr env b T) c P ⇒ Hoare P (CWhile b c) (λenv. P env ∧ (eval_bexpr env b F))) ∧ 
+  (∀ P1 Q1. (∀ env. P0 env ⇒ P1 env) ∧ Hoare P1 c Q1 ∧ (∀ env. Q1 env ⇒ Q0 env) ⇒ Hoare P0 c Q0)
 End
+
+Definition is_valid_def:
+  is_valid (P: assert) (c: com) (Q: assert) =
+  (∀ env0 env1. P env0 ∧ eval_com env0 c env1 ⇒ Q env1)
+End
+
+
+Theorem hoare_sound :
+  ∀ P c Q. Hoare P c Q ⇒ is_valid P c Q
+Proof
+  Induct_on ‘Hoare’ >> rw[]
+  (* Skip *)
+  >-(simp[is_valid_def, Once eval_com_cases])
+  (* assignment *)
+  >-()
+  (* Ceq *)
+  >-()
+  (* While *)
+  >-()
+  (* Consequence *)
+  >-()
+QED
 
 (*
 Inductive derivable : Assertion → com → Assertion → Type :=
